vale/code/arch/x64/interop/new/Vale.AsLowStar.Wrapper.fst
@@ -58,50 +58,25 @@ let core_create_lemma_disjointness
 
 let rec args_b8_lemma (args:list arg) (x:arg) 
   : Lemma
-      (requires List.memP x args)
-      (ensures 
+      (List.memP x args ==>
         (match x with
          | (| TD_Buffer bt _, x |) -> List.memP x (Interop.Adapters.args_b8 args)
          | _ -> True))
   = match args with
     | [] -> ()
     | a::q -> 
-      if StrongExcludedMiddle.strong_excluded_middle (a == x) 
-      then () 
-      else args_b8_lemma q x
+      args_b8_lemma q x
 
-[@__reduce__]
-let readable_one (s:V.va_state) (arg:arg) : prop =
-  match arg with
-  | (|TD_Buffer bt _, x |) -> 
-    ME.buffer_readable VS.(s.mem) (as_vale_buffer #(ME.TBase bt) x) /\ True
-  | _ -> True
+let readable_cons (hd:arg) (tl:list arg) (s:ME.mem)
+  : Lemma VSig.(readable (hd::tl) s <==> (readable_one s hd /\ readable tl s))
+  = BigOps.big_and'_cons VSig.(readable_one s) hd tl
 
-[@__reduce__]
-let readable (args:list arg) (s:V.va_state) : prop =
-  BigOps.big_and' (readable_one s) args
+let arg_is_registered_root (s:ME.mem) (a:arg) =
+  match a with
+  | (| TD_Buffer bt _, x |) ->
+    List.memP x (Interop.Adapters.ptrs_of_mem s)
+  | _ -> true
 
-let readable_cons (hd:arg) (tl:list arg) (s:V.va_state)
-  : Lemma 
-      (requires (readable (hd::tl) s))
-      (ensures (readable_one s hd /\ readable tl s))
-  = BigOps.big_and'_cons (readable_one s) hd tl
-
-let readable_live_one (a:arg) (h:HS.mem) (s:V.va_state)
-  : Lemma 
-      (requires
-        live_arg h a /\
-        Interop.Adapters.hs_of_mem VS.(s.mem) == h)
-      (ensures
-        readable_one s a)
-  = admit()
-  // match a with
-  //   | (| TD_Buffer bt _, x |) ->
-  //       let open Vale.AsLowStar.MemoryHelpers in
-  //       buffer_readable_reveal bt x [] h x//stack
-      
-  //   | _ -> ()
-  
 let core_create_lemma_readable
     (args:IX64.arity_ok arg)
     (h0:HS.mem)
@@ -109,30 +84,58 @@ let core_create_lemma_readable
   : Lemma
       (ensures 
         (let va_s = create_initial_vale_state args h0 stack in
-         VSig.mk_readable (arg_of_lb stack::args) va_s))
-    = 
-    let va_s = create_initial_vale_state args h0 stack in
-    let args2 = arg_of_lb stack::args in
-    let rec aux (args':list arg{forall x. List.memP x args' ==> List.memP x args2})
-                (out:VSig.sprop) 
-      : Lemma
-          (requires out va_s)
-          (ensures VSig.mk_readable_aux args' out va_s)
-      = match args' with
-        | [] -> ()
-        | a::q ->
-          match a with
-          | (| TD_Buffer bt _, x |) ->
-            begin
-              let open Vale.AsLowStar.MemoryHelpers in
-              buffer_readable_reveal bt x args h0 stack;
-              Interop.Adapters.mk_mem_injective (arg_of_lb stack::args) h0;
-              args_b8_lemma args2 a;
-              aux q (VSig.create_out_readable out bt x)
-            end
-          | _ -> aux q out
+         VSig.readable (arg_of_lb stack::args) VS.(va_s.mem)))
+  = 
+    let readable_registered_one (a:arg) (s:ME.mem)
+      : Lemma 
+          VSig.(arg_is_registered_root s a <==> readable_one s a)
+      = match a with
+        | (| TD_Buffer bt _, x |) ->
+          Vale.AsLowStar.MemoryHelpers.reveal_readable #(ME.TBase bt) x s
+        | _ -> ()
     in
-    aux args2 (fun _ -> True)
+    let rec readable_registered_all 
+        (args:list arg)
+        (s:ME.mem {forall x. List.memP x args ==> arg_is_registered_root s x})
+      : Lemma VSig.(readable args s)
+      = match args with
+        | [] -> ()
+        | hd::tl ->
+          readable_cons hd tl s;
+          readable_registered_one hd s;
+          readable_registered_all tl s
+     in
+     let readable_mk_mem
+         (args:list arg)
+         (h:mem_roots args)
+       : Lemma 
+           (let mem = Interop.Adapters.mk_mem args h in
+            VSig.readable args mem)
+       = let mem = Interop.Adapters.mk_mem args h in
+         Interop.Adapters.mk_mem_injective args h;
+         FStar.Classical.forall_intro (FStar.Classical.move_requires (args_b8_lemma args));
+         readable_registered_all args mem
+     in
+     readable_mk_mem (arg_of_lb stack::args) h0
+
+let readable_live_one (m:ME.mem) (a:arg)
+  : Lemma (VSig.readable_one m a ==>
+           live_arg (Interop.Adapters.hs_of_mem m) a)
+  = match a with
+    | (| TD_Buffer bt _, x |) ->
+      Vale.AsLowStar.MemoryHelpers.readable_live #(ME.TBase bt) x m
+    | _ -> ()
+
+let rec readable_all_live (m:ME.mem) (args:list arg)
+  : Lemma (VSig.readable args m ==>
+           all_live (Interop.Adapters.hs_of_mem m) args)
+  = match args with
+    | [] -> ()
+    | hd::tl ->
+      readable_cons hd tl m;
+      all_live_cons hd tl (Interop.Adapters.hs_of_mem m);
+      readable_live_one m hd;
+      readable_all_live m tl
 
 let core_create_lemma_readable2
     (args:IX64.arity_ok arg)
@@ -141,29 +144,10 @@ let core_create_lemma_readable2
   : Lemma
       (ensures 
         (let va_s = create_initial_vale_state args h0 stack in
-         VSig.mk_readable args va_s))
-  = 
+         VSig.readable args VS.(va_s.mem)))
+  = core_create_lemma_readable args h0 stack;
     let va_s = create_initial_vale_state args h0 stack in
-    let rec aux (args':list arg{forall x. List.memP x args' ==> List.memP x args})
-                (out:VSig.sprop)
-      : Lemma
-          (requires out va_s)
-          (ensures VSig.mk_readable_aux args' out va_s)
-      = match args' with
-        | [] -> ()
-        | a::q ->
-          match a with
-          | (| TD_Buffer bt _, x |) ->
-            begin
-              let open Vale.AsLowStar.MemoryHelpers in
-              buffer_readable_reveal bt x args h0 stack;
-              Interop.Adapters.mk_mem_injective (arg_of_lb stack::args) h0;
-              args_b8_lemma (arg_of_lb stack::args) a;
-              aux q (VSig.create_out_readable out bt x)
-            end
-        | _ -> aux q out
-    in 
-    aux args (fun _ -> True)
+    readable_cons (arg_of_lb stack) args VS.(va_s.mem)
     
 let core_create_lemma_mem_correspondance
     (args:IX64.arity_ok arg)
@@ -312,7 +296,7 @@ let core_create_lemma
          fst (IX64.create_initial_trusted_state args h0 stack) == SL.state_to_S va_s /\
          LSig.mem_correspondence args h0 va_s /\
          LSig.mk_vale_disjointness stack args /\
-         VSig.mk_readable args va_s /\
+         VSig.readable args VS.(va_s.mem) /\
          LSig.vale_pre_hyp stack args va_s))
   = let va_s = create_initial_vale_state args h0 stack in
     core_create_lemma_mem_correspondance args h0 stack;
@@ -504,9 +488,10 @@ let vale_lemma_as_prediction
        pop_is_popped h1_pre_pop;
        assert (HS.popped h1_pre_pop h2);
        B.popped_modifies h1_pre_pop h2;
-       assert (VSig.mk_readable args va_s1);
+       assert (VSig.readable args VS.(va_s1.mem));
        assert (disjoint_or_eq args);
-       assume (all_live h1_pre_pop args);
+       readable_all_live VS.(va_s1.mem) args;
+       assert (all_live h1_pre_pop args);
        assert (mem_roots_p h1_pre_pop args);
        frame_mem_correspondence args h1_pre_pop h2 va_s1 (B.loc_regions false (Set.singleton (HS.get_tip h1_pre_pop)));
        assert (B.modifies (loc_modified_args args) alloc_push_h0 h1_pre_pop);
